WIP

src/WFLib.v
@@ -254,9 +254,8 @@ Section WFTYPE.
 End WFTYPE.
 
 Definition ord_tree_WF {A}: WF := mk_wf (@ord_tree_lt_well_founded A).
-
 Definition option_WF (A: WF): WF := mk_wf (option_lt_well_founded A.(wf)).
 Definition sum_WF (A B: WF): WF := mk_wf (sum_lt_well_founded A.(wf) B.(wf)).
 Definition prod_WF (A B: WF): WF := mk_wf (prod_lt_well_founded A.(wf) B.(wf)).
-
 Definition clos_trans_WF (A: WF): WF := mk_wf (clos_trans_well_founded A.(wf)).
+Definition double_rel_WF (A B: WF): WF := mk_wf (double_rel_well_founded A.(wf) B.(wf)).
