src/YOrd2Stid.v
@@ -9,8 +9,132 @@ Export ITreeNotations.
 
 From Fairness Require Import Axioms.
 From Fairness Require Export ITreeLib FairBeh FairSim NatStructs.
-From Fairness Require Import pind PCM World WFLib.
+From Fairness Require Import pind PCM World WFLib ThreadsURA.
 From Fairness Require Import Mod ModSimYOrd ModSimStid.
 
 Set Implicit Arguments.
 
+Section IMAPAUX1.
+
+  Variable wf: WF.
+
+  Definition imap_proj_id1 {id1 id2: ID} (im: @imap (id_sum id1 id2) wf): @imap id1 wf := fun i => im (inl i).
+  Definition imap_proj_id2 {id1 id2: ID} (im: @imap (id_sum id1 id2) wf): @imap id2 wf := fun i => im (inr i).
+  Definition imap_proj_id {id1 id2: ID} (im: @imap (id_sum id1 id2) wf): prod (@imap id1 wf) (@imap id2 wf) :=
+    (imap_proj_id1 im, imap_proj_id2 im).
+
+  Definition imap_sum_id {id1 id2: ID} (im: prod (@imap id1 wf) (@imap id2 wf)): @imap (id_sum id1 id2) wf :=
+    fun i => match i with | inl il => (fst im) il | inr ir => (snd im) ir end.
+
+  Lemma imap_sum_proj_id_inv1
+        id1 id2
+        (im1: @imap id1 wf)
+        (im2: @imap id2 wf)
+    :
+    imap_proj_id (imap_sum_id (im1, im2)) = (im1, im2).
+  Proof. reflexivity. Qed.
+
+  Lemma imap_sum_proj_id_inv2
+        id1 id2
+        (im: @imap (id_sum id1 id2) wf)
+    :
+    imap_sum_id (imap_proj_id im) = im.
+  Proof. extensionality i. unfold imap_sum_id. des_ifs. Qed.
+
+End IMAPAUX1.
+Global Opaque imap_proj_id1.
+Global Opaque imap_proj_id2.
+Global Opaque imap_sum_id.
+
+
+Section IMAPAUX2.
+
+  Variable id: ID.
+
+  Definition imap_proj_wf1 {wf1 wf2: WF} (im: @imap id (double_rel_WF wf1 wf2)): @imap id wf1 := fun i => fst (im i).
+  Definition imap_proj_wf2 {wf1 wf2: WF} (im: @imap id (double_rel_WF wf1 wf2)): @imap id wf2 := fun i => snd (im i).
+  Definition imap_proj_wf {wf1 wf2: WF} (im: @imap id (double_rel_WF wf1 wf2)): prod (@imap id wf1) (@imap id wf2) :=
+    (imap_proj_wf1 im, imap_proj_wf2 im).
+
+  Definition imap_sum_wf {wf1 wf2: WF} (im: prod (@imap id wf1) (@imap id wf2)): @imap id (double_rel_WF wf1 wf2) :=
+    fun i => (fst im i, snd im i).
+
+  Lemma imap_sum_proj_wf_inv1
+        wf1 wf2
+        (im1: @imap id wf1)
+        (im2: @imap id wf2)
+    :
+    imap_proj_wf (imap_sum_wf (im1, im2)) = (im1, im2).
+  Proof. reflexivity. Qed.
+
+  Lemma imap_sum_proj_wf_inv2
+        wf1 wf2
+        (im: @imap id (double_rel_WF wf1 wf2))
+    :
+    imap_sum_wf (imap_proj_wf im) = im.
+  Proof.
+    extensionality i. unfold imap_sum_wf, imap_proj_wf, imap_proj_wf1, imap_proj_wf2. ss. destruct (im i); ss.
+  Qed.
+
+End IMAPAUX2.
+Global Opaque imap_proj_wf1.
+Global Opaque imap_proj_wf2.
+Global Opaque imap_sum_wf.
+
+
+
+Section PROOF.
+
+  Context `{M: URA.t}.
+
+  Variable state_src: Type.
+  Variable state_tgt: Type.
+
+  Variable ident_src: ID.
+  Variable _ident_tgt: ID.
+  Let ident_tgt := sum_tid _ident_tgt.
+
+  Variable wf_src: WF.
+  Variable wf_tgt: WF.
+
+  Let srcE := ((@eventE ident_src +' cE) +' sE state_src).
+  Let tgtE := ((@eventE _ident_tgt +' cE) +' sE state_tgt).
+
+  Let shared :=
+        (TIdSet.t *
+           (@imap ident_src wf_src) *
+           (@imap ident_tgt wf_tgt) *
+           state_src *
+           state_tgt)%type.
+  Let shared_rel: Type := shared -> Prop.
+  Variable I: shared -> URA.car -> Prop.
+
+  Variable wf_stt: Type -> Type -> WF.
+
+
+  Let ident_src2 := sum_tid ident_src.
+
+  Let wf_src_th {R0 R1}: WF := prod_WF (prod_WF (wf_stt R0 R1) wf_tgt) (nm_wf (wf_stt R0 R1)).
+  Let wf_src2 {R0 R1}: WF := double_rel_WF (@wf_src_th R0 R1) wf_src.
+
+  Let srcE2 := ((@eventE ident_src2 +' cE) +' sE state_src).
+  Let shared2 {R0 R1} :=
+        (TIdSet.t *
+           (@imap ident_src2 (@wf_src2 R0 R1)) *
+           (@imap ident_tgt wf_tgt) *
+           state_src *
+           state_tgt)%type.
+  Let shared2_rel {R0 R1}: Type := (@shared2 R0 R1) -> Prop.
+
+  Let M2 {R0 R1}: URA.t := URA.prod (@thsRA (prod_WF (wf_stt R0 R1) (wf_stt R0 R1)).(T)) M.
+
+  Definition I2 {R0 R1}: (@shared2 R0 R1) -> (@URA.car (@M2 R0 R1)) -> Prop :=
+    fun '(ths, im_src, im_tgt, st_src, st_tgt) '(ths_r, r) =>
+      (<<INV: I (ths, imap_proj_wf2 (imap_proj_id2 im_src), im_tgt, st_src, st_tgt) r>>)
+  /\
+        (<<>>)
+
+    Variable I: shared -> URA.car -> Prop.
+
+
+End PROOF.
